Test.Float.Lemmas.Arithmetic.fst
@@ -12,11 +12,11 @@ let to_of_inj (p: pair) : Lemma (to_pair (of_pair p) = p) [SMTPat (of_pair p)]
 let commut_add a b : Lemma (a +. b = b +. a) = ()
 let commut_mul a b : Lemma (a *. b = b *. a) = ()
 
-let add_zero a : Lemma (a +. zero = a /\ zero +. a = a) = ()
-let sub_zero a : Lemma (a -. zero = a) = ()
-let sub_self a : Lemma (a -. a = zero) = ()
-let mul_one  a : Lemma (a *. one = a /\ one *. a = a) = ()
-let mul_zero a : Lemma (a *. zero = zero /\ zero *. a = zero) = ()
+let add_zero a : Lemma (a +. _0 = a /\ _0 +. a = a) = ()
+let sub_zero a : Lemma (a -. _0 = a) = ()
+let sub_self a : Lemma (a -. a = _0) = ()
+let mul_one  a : Lemma (a *. _1 = a /\ _1 *. a = a) = ()
+let mul_zero a : Lemma (a *. _0 = _0 /\ _0 *. a = _0) = ()
 
 let sub_is_add_neg a b : Lemma (a -. b = a +. (~.b)) = 
   let a', b', exp_min = to_shared_exp a b in
@@ -24,11 +24,11 @@ let sub_is_add_neg a b : Lemma (a -. b = a +. (~.b)) =
   assert (_a' = a');
   assert (_b' = -b');
   assert (exp_min = exp_min)
-let neg_is_mul_neg_one a : Lemma (~.a = (~.one) *. a /\ ~.a = a *. (~.one)) = ()
+let neg_is_mul_neg_one a : Lemma (~.a = (~._1) *. a /\ ~.a = a *. (~._1)) = ()
 let double_neg a : Lemma (~.(~.a) = a) = ()
-let neg_is_zero_sub a : Lemma (~.a = zero -. a) =
+let neg_is_zero_sub a : Lemma (~.a = _0 -. a) =
   add_zero (~.a);
-  sub_is_add_neg zero (~.a)
+  sub_is_add_neg _0 (~.a)
 
 let assoc_add_left a b c : 
   Lemma (a +. b +. c = (a +. b) +. c /\
@@ -54,7 +54,7 @@ let distrib_neg_add a b : Lemma (~.(a +. b) = ~.a +. ~.b /\
   = 
   let aux a b : Lemma (~.(a +. b) = ~.a +. ~.b) =
     neg_is_mul_neg_one (a +. b);
-    distrib_add (~.one) a b;
+    distrib_add (~._1) a b;
     neg_is_mul_neg_one a;
     neg_is_mul_neg_one b
   in
@@ -73,7 +73,7 @@ let distrib_neg_mul a b : Lemma (~.(a *. b) = (~.a) *. b /\
                                  ~.(a *. b) = a *. (~.b)) =
   let aux a b : Lemma (~.(a *. b) = (~.a) *. b) =
     neg_is_mul_neg_one (a *. b); 
-    assoc_mul_right ~.one a b;
+    assoc_mul_right ~._1 a b;
     neg_is_mul_neg_one a
   in aux a b; aux b a
 
