Test.Float.Trigonometry.fsti
@@ -6,30 +6,30 @@ open Test.Float.Lemmas.Inequality
 
 
 val _180 : (x: float{x = of_int 180})
-val _90 : (x: float{x = of_int 90})
+val _90  : (x: float{x = of_int 90})
 
-val sin : float -> (r: float{r.[~.one, one]})
-val cos : float -> (r: float{r.[~.one, one]})
+val sin : float -> (r: float{r.[~._1, _1]})
+val cos : float -> (r: float{r.[~._1, _1]})
 val arctg (x y: float) : (r: float{r.[~._180, _180]})
-val hypot (x y: float) : (r: float{r *. r = x *. x +. y *. y /\ r >=. zero})
+val hypot (x y: float) : (r: float{r *. r = x *. x +. y *. y /\ r >=. _0})
 
 val sin_odd  (a: float) : Lemma (sin a = ~.(sin ~.a))
 val cos_even (a: float) : Lemma (cos a = cos ~.a)
-val arctg_x_pos (x y: float) : Lemma (requires x >=. zero) (ensures (arctg x y).(~._90, _90)) [SMTPat (arctg x y)]
+val arctg_x_pos (x y: float) : Lemma (requires x >=. _0) (ensures (arctg x y).(~._90, _90)) [SMTPat (arctg x y)]
 
-val sin_0 (a: float{a = zero}) : Lemma (sin a = zero)
-val cos_0 (a: float{a = zero}) : Lemma (cos a = one)
-let sin_cos_0 (a: float{a = zero}) : Lemma (sin a = zero /\ cos a = one) = sin_0 a; cos_0 a
+val sin_0 (a: float{a = _0}) : Lemma (sin a = _0)
+val cos_0 (a: float{a = _0}) : Lemma (cos a = _1)
+let sin_cos_0 (a: float{a = _0}) : Lemma (sin a = _0 /\ cos a = _1) = sin_0 a; cos_0 a
 
-val sin_90 (a: float{a = of_int 90}) : Lemma (sin a = one)
-val cos_90 (a: float{a = of_int 90}) : Lemma (cos a = zero)
-let sin_cos_90 (a: float{a = of_int 90}) : Lemma (sin a = one /\ cos a = zero) = sin_90 a; cos_90 a
+val sin_90 (a: float{a = of_int 90}) : Lemma (sin a = _1)
+val cos_90 (a: float{a = of_int 90}) : Lemma (cos a = _0)
+let sin_cos_90 (a: float{a = of_int 90}) : Lemma (sin a = _1 /\ cos a = _0) = sin_90 a; cos_90 a
 
-val osn_trig_todj (a: float) : Lemma ((sin a *. sin a) +. (cos a *. cos a) = one) 
+val osn_trig_todj (a: float) : Lemma ((sin a *. sin a) +. (cos a *. cos a) = _1) 
 
 val cos_add (a b: float) : Lemma (cos (a +. b) = cos a *. cos b -. sin a *. sin b)
 val sin_add (a b: float) : Lemma (sin (a +. b) = sin a *. cos b +. cos a *. sin b)
 
-val arctg_of_cos_sin (a: float{a.[~._180, _180]}) (b: notzero) : Lemma (arctg (b *. cos a) (b *. sin a) = a)
+val arctg_of_cos_sin (a: float{a.[~._180, _180]}) (b: not_0) : Lemma (arctg (b *. cos a) (b *. sin a) = a)
 
-val cos_pos (a: float{a.(~._90, _90)}) : Lemma (cos a >. zero)
+val cos_pos (a: float{a.(~._90, _90)}) : Lemma (cos a >. _0)
